working on d_conj_set lemm for concrete gba

examples/logic/ltl/generalHelpersScript.sml
@@ -1,4 +1,4 @@
-open HolKernel Parse bossLib boolLib pred_setTheory relationTheory set_relationTheory arithmeticTheory pairTheory listTheory optionTheory prim_recTheory whileTheory
+open HolKernel Parse bossLib boolLib pred_setTheory relationTheory set_relationTheory arithmeticTheory pairTheory listTheory optionTheory prim_recTheory whileTheory rich_listTheory
 
 val _ = new_theory "generalHelpers"
 
@@ -147,6 +147,18 @@ val char_def = Define `char Σ p = { a | (a ∈ Σ) /\ (p ∈ a)}`;
 
 val char_neg_def = Define `char_neg Σ p = Σ DIFF (char Σ p)`;
 
+val CHAR_LEMM = store_thm
+  ("CHAR_LEMM",
+   ``!Σ x. char Σ x ⊆ Σ``,
+   fs[char_def,SUBSET_DEF] >> rpt strip_tac
+  );
+
+val CHAR_NEG_LEMM = store_thm
+  ("CHAR_NEG_LEMM",
+   ``!Σ x. char_neg Σ x ⊆ Σ``,
+   fs[char_neg_def,DIFF_SUBSET]
+  );
+
 val d_conj_def = Define
   `d_conj d1 d2 = { (a1 ∩ a2, e1 ∪ e2) | ((a1,e1) ∈ d1) /\ ((a2,e2) ∈ d2)}`;
 
@@ -262,6 +274,233 @@ val D_CONJ_SET_LEMM2 = store_thm
   rpt strip_tac >> metis_tac[D_CONJ_SET_LEMM]
   );
 
+val D_CONJ_SET_LEMM3 = store_thm
+  ("D_CONJ_SET_LEMM3",
+   ``!s A a a' e'. FINITE s
+        ∧ (!q d. (q,d) ∈ s ==> (a' q,e' q) ∈ d ∧ a ⊆ a' q)
+        ∧ (a ⊆ A)
+     ==> (A ∩ BIGINTER {a' q | q ∈ IMAGE FST s },
+          BIGUNION {e' q | q ∈ IMAGE FST s})
+                      ∈ d_conj_set s A``,
+    `!s. FINITE (s:α # ((β -> bool) # (γ -> bool) -> bool) -> bool)
+        ==>
+         (!A a a' e'. (!q d. (q,d) ∈ s  ==> (a' q,e' q) ∈ d ∧ a ⊆ a' q)
+                  ∧ (a ⊆ A)
+          ==> (A ∩ BIGINTER {a' q | q ∈ IMAGE FST s },
+               BIGUNION {e' q | q ∈ IMAGE FST s}) ∈ d_conj_set s A)`
+    suffices_by metis_tac[]
+    >> Induct_on `s` >> rpt strip_tac >> fs[]
+     >- fs[d_conj_set_def,ITSET_THM]
+     >- (`(A ∩ BIGINTER {a' q | ?x. (q = FST x) ∧ x ∈ s},
+           BIGUNION {e' q | ?x. (q = FST x) ∧ x ∈ s}) ∈ d_conj_set s A`
+            by metis_tac[]
+         >> simp[d_conj_set_def]
+         >> `s DELETE e = s` by fs[DELETE_NON_ELEMENT_RWT]
+         >> imp_res_tac D_CONJ_SET_RECURSES
+         >> first_x_assum (qspec_then `e` mp_tac) >> rpt strip_tac
+         >> first_x_assum (qspec_then `{(A,{})}` mp_tac)
+         >> rpt strip_tac >> fs[] >> fs[d_conj_set_def]
+         >> simp[d_conj_def] >> qexists_tac `a' (FST e)`
+         >> qexists_tac `A ∩ BIGINTER {a' q | q ∈ IMAGE FST s }`
+         >> qexists_tac `e' (FST e)`
+         >> qexists_tac `BIGUNION {e' q | q ∈ IMAGE FST s }`
+         >> rpt strip_tac
+         >> simp[IN_IMAGE] >> dsimp[] >> simp[SET_EQ_SUBSET,SUBSET_DEF,IN_BIGINTER]
+         >> rpt strip_tac >> metis_tac[]
+        )
+  );
+
+val MEM_SUBSET_def = Define`
+    (MEM_SUBSET [] l = T)
+  ∧ (MEM_SUBSET (h::ls) l = (MEM h l ∧ MEM_SUBSET ls l))`;
+
+val MEM_SUBSET_SET_TO_LIST = store_thm
+  ("MEM_SUBSET_SET_TO_LIST",
+   ``!l1 l2. MEM_SUBSET l1 l2 = (set l1 ⊆ set l2)``,
+   Induct_on `l1` >> fs[MEM_SUBSET_def] >> rpt strip_tac
+  );
+
+val MEM_SUBSET_REFL = store_thm
+  ("MEM_SUBSET_REFL",
+   ``!l. MEM_SUBSET l l``,
+   Induct_on `l` >> fs[MEM_SUBSET_def] >> rpt strip_tac
+   >> metis_tac[MEM_SUBSET_SET_TO_LIST,SUBSET_DEF,MEM]
+  );
+
+val MEM_SUBSET_APPEND = store_thm
+  ("MEM_SUBSET_APPEND",
+   ``!l1 l2. MEM_SUBSET l1 (l1++l2)
+           ∧ MEM_SUBSET l2 (l1++l2)``,
+   rpt strip_tac
+   >> metis_tac[MEM_SUBSET_SET_TO_LIST,SUBSET_DEF,MEM,MEM_APPEND]
+  );
+
+val MEM_SUBSET_TRANS = store_thm
+  ("MEM_SUBSET_TRANS",
+   ``!l1 l2 l3. MEM_SUBSET l1 l2 ∧ MEM_SUBSET l2 l3 ==> MEM_SUBSET l1 l3``,
+   metis_tac[MEM_SUBSET_SET_TO_LIST,SUBSET_TRANS]
+  );
+
+val MEM_EQUAL_def = Define`
+  (MEM_EQUAL l1 l2 = (MEM_SUBSET l1 l2 ∧ MEM_SUBSET l2 l1))`;
+
+val MEM_EQUAL_SET = store_thm
+  ("MEM_EQUAL_SET",
+   ``!l1 l2. MEM_EQUAL l1 l2 ==> (set l1 = set l2)``,
+   metis_tac[MEM_SUBSET_SET_TO_LIST,SET_EQ_SUBSET,MEM_EQUAL_def]
+  );
+
+(* val REM_RIGHT_def = Define` *)
+(*     (REM_RIGHT x [] = ([], F)) *)
+(*   ∧ (REM_RIGHT x (h::ls) = *)
+(*      if h = x *)
+(*      then (ls,T) *)
+(*      else REM_RIGHT x ls *)
+(*     )`; *)
+
+(* val REM_RIGHT_SND_LEMM = store_thm *)
+(*   ("REM_RIGHT_LEMM", *)
+(*    ``!x l. (SND (REM_RIGHT x l) = (MEM x l))``, *)
+(*    Induct_on `l` >> fs[REM_RIGHT_def] >> rpt strip_tac *)
+(*    >> Cases_on `x = h` >> fs[] *)
+(*   ); *)
+
+(* val MEM_EQUAL_def = Define` *)
+(*    (MEM_EQUAL [] [] = T) *)
+(*  ∧ (MEM_EQUAL (h::ls) [] = F) *)
+(*  ∧ (MEM_EQUAL [] (h::ls) = F) *)
+(*  ∧ (MEM_EQUAL (h1::ls1) (h2::ls2) = *)
+(*     let (rest,mem) = REM_RIGHT h1 ls2 *)
+(*     in if mem *)
+(*        then MEM_EQUAL ls1 rest *)
+(*        else F *)
+(*    )`; *)
+
+(* val MEM_EQUAL_AD_SYMM = store_thm *)
+(*   ("MEM_EQUAL_AD_SYMM", *)
+(*    ``!l1 l2. ALL_DISTINCT l1 ∧ ALL_DISTINCT l2 *)
+(*        ==> (MEM_EQUAL l1 l2 = MEM_EQUAL l2 l1 *)
+(*           ∧ (MEM_EQUAL l1 l2 = (set l1 = set l2)))``, *)
+(*    Induct_on `l2` >> rpt strip_tac >> fs[MEM_EQUAL_def] *)
+(*    >- (Cases_on `l1` >> fs[MEM_EQUAL_def]) *)
+(*    >- (Cases_on `l1` >> fs[MEM_EQUAL_def]) *)
+(*    >- (Cases_on `l1` >> simp[MEM_EQUAL_def] >> fs[] *)
+(*        >> `MEM_EQUAL t l2 = MEM_EQUAL l2 t *)
+(*          ∧ MEM_EQUAL t l2 = (set t = set l2)` by metis_tac[] *)
+(*        >> Cases_on `MEM_EQUAL t l2` *)
+(*        >- (fs[] *)
+(*            >> `~SND (REM_RIGHT h' l2)` by metis_tac[MEM,REM_RIGHT_SND_LEMM] *)
+(*            >> `~SND (REM_RIGHT h t)` by metis_tac[MEM,REM_RIGHT_SND_LEMM] *)
+(*            >> Cases_on `REM_RIGHT h' l2` >> Cases_on `REM_RIGHT h t` >> fs[] *)
+(*           ) *)
+(*        >- (fs[] >> qabbrev_tac `R_t = FST (REM_RIGHT h t)` *)
+(*            >> `~(MEM_EQUAL l2 R_t) *)
+
+
+(*            >> `?x. (MEM x t ∧ ~MEM x l2) \/ (~MEM x t ∧ MEM x l2)` *)
+(*                 by (CCONTR_TAC >> fs[] *)
+(*                     >> `!x. MEM x t = MEM x l2` by metis_tac[] *)
+(*                     >> `set t = set l2` *)
+(*                        by (PURE_REWRITE_TAC[SET_EQ_SUBSET,SUBSET_DEF] *)
+(*                            >> rpt strip_tac >> metis_tac[MEM] *)
+(*                           ) *)
+(*                     >- (`~(h' = x)` by metis_tac[] >> fs[] *)
+
+
+
+(*                         >> Cases_on `x = h` >> fs[] *)
+(*                         >- (rw[] >> ) *)
+(*                        ) *)
+(*                    ) *)
+(*            ) *)
+(*        ) *)
+(*    >- (Cases_on `l1` >> fs[MEM_EQUAL_def] >> ) *)
+
+
+(* ) *)
+
+(* Cases_on `MEM x t` >> fs[] >> ) *)
+(* ) *)
+
+
+(* ) *)
+(* ) *)
+
+
+(* ) *)
+
+
+
+(* val MEM_EQUAL_AD_SET = store_thm *)
+(*   ("MEM_EQUAL_ALL_DISTINCT", *)
+(*  ``!ls1 ls2. ALL_DISTINCT ls1 ∧ ALL_DISTINCT ls2 *)
+(*         ==> (MEM_EQUAL ls1 ls2 = (set ls1 = set ls2))``, *)
+(*  simp[EQ_IMP_THM] >> rpt strip_tac *)
+(*  >- () *)
+
+
+
+(* ) *)
+
+val ALL_DISTINCT_PAIRS_LEMM = store_thm
+  ("ALL_DISTINCT_PAIRS_LEMM",
+   ``!x y1 y2 l.
+     ALL_DISTINCT (MAP FST l)
+     ∧ (MEM (x,y1) l)
+     ∧ (MEM (x,y2) l)
+     ==> (y1 = y2)``,
+   Induct_on `l` >> fs[ALL_DISTINCT] >> rpt strip_tac
+   >- (Cases_on `h` >> fs[])
+   >- (fs[MEM_MAP] >> Cases_on `h` >> fs[] >> rw[]
+       >> first_x_assum (qspec_then `(q,y2)` mp_tac) >> fs[])
+   >- (fs[MEM_MAP] >> Cases_on `h` >> fs[] >> rw[]
+       >> first_x_assum (qspec_then `(q,y1)` mp_tac) >> fs[])
+   >- metis_tac[]
+  );
+
+val FOLDR_INTER = store_thm
+  ("FOLDR_INTER",
+   ``!f A l.
+  (!x. MEM x l
+       ==> (FOLDR (λa sofar. f a ∩ sofar) A l
+                  ⊆ f x))
+  ∧ (FOLDR (λa sofar. f a ∩ sofar) A l
+           ⊆ A)``,
+   Induct_on `l` >> rpt strip_tac >> fs[]
+   >> metis_tac[INTER_SUBSET,SUBSET_TRANS]
+  );
+
+val FOLDR_APPEND = store_thm
+  ("FOLDR_APPEND",
+   ``!f A l.
+  (!x. MEM x l
+       ==> MEM_SUBSET (f x) (FOLDR (λa sofar. f a ++ sofar) A l))
+  ∧ (MEM_SUBSET A (FOLDR (λa sofar. f a ++ sofar) A l))
+  ∧ (set (FOLDR (λa sofar. f a ++ sofar) A l) =
+     set A ∪ BIGUNION {set (f a) | MEM a l })``,
+   Induct_on `l` >> rpt strip_tac >> fs[]
+   >- fs[MEM_SUBSET_REFL]
+   >- fs[MEM_SUBSET_APPEND]
+   >- metis_tac[MEM_SUBSET_APPEND,MEM_SUBSET_TRANS]
+   >- metis_tac[MEM_SUBSET_APPEND,MEM_SUBSET_TRANS]
+   >- (simp[SET_EQ_SUBSET,SUBSET_DEF] >> rpt strip_tac >> fs[]
+       >> metis_tac[]
+      )
+  );
+
+val ZIP_MAP = store_thm
+  ("ZIP_MAP",
+   ``!l. ZIP (MAP FST l, MAP SND l) = l``,
+   Induct_on `l` >> fs[ZIP]
+  );
+
+val MAP_LEMM = store_thm
+  ("MAP_LEMM",
+   ``!l f h a. ~MEM h l
+             ==> (MAP (λq. if q = h then a else f q) l = MAP f l)``,
+   Induct_on `l` >> rpt strip_tac >> fs[]
+  );
+
 val CAT_OPTIONS_def = Define`
    (CAT_OPTIONS [] = [])
  ∧ (CAT_OPTIONS (SOME v::ls) = v::(CAT_OPTIONS ls))
@@ -306,6 +545,86 @@ val LIST_INTER_def = Define`
   ∧ (LIST_INTER (x::xs) ls = if MEM x ls
                              then x::(LIST_INTER xs ls)
                              else LIST_INTER xs ls)`;
+
+(* val GROUP_BY_def = tDefine "GROUP_BY" *)
+(*   `(GROUP_BY P [] = []) *)
+(*  ∧ (GROUP_BY P (x::xs) = *)
+(*        (FILTER (P x) (x::xs))::(GROUP_BY P (FILTER ($~ o (P x)) xs)) *)
+(*    )` *)
+(*   (WF_REL_TAC `measure (LENGTH o SND)` >> rpt strip_tac >> fs[] *)
+(*    >> Q.HO_MATCH_ABBREV_TAC `A < SUC B` >> `A <= B ` suffices_by simp[] *)
+(*    >> metis_tac[LENGTH_FILTER_LEQ] *)
+(*   ); *)
+
+(* val GROUP_BY_SET_LEMM = store_thm *)
+(*   ("GROUP_BY_SET_LEMM", *)
+(*    ``!P l. (!x. P x x) ==> set l = (set (FLAT (GROUP_BY P l)))``, *)
+(*    Induct_on `l` >> fs[GROUP_BY_def] >> rpt strip_tac *)
+(*    >> Cases_on `P h h` >> fs[] *)
+(*    >- () *)
+
+(* ) *)
+
+val SPAN_def = Define`
+   (SPAN R [] = ([],[]))
+ ∧ (SPAN R (x::xs) =
+    if R x
+    then (let (ys,rs) = SPAN R xs
+          in (x::ys,rs))
+    else ([],x::xs)
+   )`;
+
+val SPAN_APPEND = store_thm
+  ("SPAN_APPEND",
+   ``!R l l1 l2. (SPAN R l = (l1,l2)) ==> (l1 ++ l2 = l)``,
+   gen_tac >> Induct_on `l` >> fs[SPAN_def] >> rpt strip_tac
+   >> Cases_on `R h` >> fs[]
+   >> Cases_on `SPAN R l` >> rw[] >> fs[]
+  );
+
+val GROUP_BY_def = tDefine "GROUP_BY"
+  `(GROUP_BY P []  = [])
+ ∧ (GROUP_BY P (x::xs) =
+    let (ys,rs) = SPAN (P x) (xs)
+    in (x::ys)::(GROUP_BY P rs)
+   )`
+   (WF_REL_TAC `measure (LENGTH o SND)` >> rpt strip_tac
+    >> `ys ++ rs = xs` by metis_tac[SPAN_APPEND]
+    >> `LENGTH ys + LENGTH rs = LENGTH xs` by metis_tac[LENGTH_APPEND]
+    >> fs[]
+   );
+
+val GROUP_BY_FLAT = store_thm
+  ("GROUP_BY_FLAT",
+   ``!P l. set (FLAT (GROUP_BY P l)) = set l``,
+   gen_tac
+   >> `!l1 l2 l. (l1 ++ l2 = l)
+                 ==> (set (FLAT (GROUP_BY P l2)) = set l2)` by (
+       Induct_on `l` >> fs[GROUP_BY_def] >> rpt strip_tac
+       >> Cases_on `l1`
+       >- (fs[] >> simp[GROUP_BY_def] >> Cases_on `SPAN (P h) l`
+           >> `q ++ r = l` by metis_tac[SPAN_APPEND]
+           >> fs[] >> `set (FLAT (GROUP_BY P r)) = set r` by metis_tac[]
+           >> rw[LIST_TO_SET_APPEND]
+          )
+       >- (Cases_on `l2` >> fs[GROUP_BY_def] >> rw[]
+           >> Cases_on `SPAN (P h'') t'` >> fs[]
+           >> `q++r = t'` by metis_tac[SPAN_APPEND]
+           >> first_x_assum (qspec_then `t ++ [h''] ++ q` mp_tac) >> simp[]
+           >> rpt strip_tac >> rw[LIST_TO_SET_APPEND]
+          )
+   )
+   >> `[] ++ l = l` by simp[] >> metis_tac[]
+  );
+
+val ONLY_MINIMAL_def = Define`
+    (ONLY_MINIMAL P [] = [])
+  ∧ (ONLY_MINIMAL P (x::xs) =
+      if EXISTS (λx1. P x1 x) xs
+      then ONLY_MINIMAL P xs
+      else x::(ONLY_MINIMAL P xs)
+    )`;
+
 
 val INDEX_FIND_LEMM = store_thm
   ("INDEX_FIND_LEMM",
